pcuic/theories/PCUICSize.v
@@ -21,8 +21,10 @@ Fixpoint size t : nat :=
   | tApp u v => S (size u + size v)
   | tProd na A B => S (size A + size B)
   | tLetIn na b t b' => S (size b + size t + size b')
-  | tCase ind p c brs => S (list_size size p.(pparams) + size p.(preturn) + 
-    size c + list_size (size ∘ bbody) brs)
+  | tCase ind p c brs => S (list_size size p.(pparams) + 
+    context_size size p.(pcontext) +
+    size p.(preturn) + 
+    size c + list_size (fun br => context_size size br.(bcontext) + size (bbody br)) brs)
   | tProj p c => S (size c)
   | tFix mfix idx => S (mfixpoint_size size mfix)
   | tCoFix mfix idx => S (mfixpoint_size size mfix)
